Temp commit using iter. Potential Catch 22

src/Util/Streams.dfy
@@ -4,151 +4,74 @@ module Streams {
   import opened StandardLibrary
   import opened UInt = StandardLibrary.UInt
 
-  class MemoryReader<T> {
-    ghost var Repr: set<object>
-    const data: seq<T>
-    var pos: nat
-
-    predicate Valid() reads this, Repr
+  iterator SeqIter<T>(s: seq<T>) yields (x : T)
+    yield ensures x in s
+    yield ensures |xs| <= |s|
+    yield ensures xs == s[..|xs|]
+    yield ensures fresh(_new)
+    ensures fresh(_new)
+  {
+    var idx := 0;
+    while idx < |s|
+      invariant 0 <= idx <= |s|
+      invariant idx == |xs|
+      invariant xs <= s
     {
-      Repr == {this} &&
-      pos <= |data|
-    }
-
-    constructor(s: seq<T>)
-      ensures pos == 0
-      ensures data[..] == s
-      ensures Valid()
-      ensures fresh(Repr - {this})
-    {
-      this.data := s;
-      this.pos := 0;
-      Repr := {this};
-    }
-
-    method ReadBytes(byteCount: nat) returns (bytes: seq<T>)
-      requires byteCount + pos <= |data|
-      requires Valid()
-      modifies Repr
-      ensures byteCount == 0 ==> bytes == []
-      ensures byteCount > 0 ==> bytes == data[old(pos)..][..byteCount]
-      ensures pos == old(pos) + byteCount
-      ensures Valid()
-      ensures fresh(Repr - old(Repr))
-    {
-      bytes := data[pos..][..byteCount];
-      pos := pos + byteCount;
-      Repr := {this};
-      return bytes;
-    }
-
-    method ReadExact(n: nat) returns (res: Result<seq<T>>)
-      requires Valid()
-      modifies Repr
-      ensures res.Success? ==> |res.value| == n
-      ensures res.Failure? ==> n > |data| - pos
-      ensures Valid()
-      ensures fresh(Repr - old(Repr))
-    {
-      if n > |data| - pos {
-        return Failure("IO Error: Not enough bytes left on stream.");
-      } else {
-        var bytes := ReadBytes(n);
-        Repr := {this};
-        return Success(bytes);
-      }
+      x := s[idx];
+      yield;
+      idx := idx + 1;
     }
   }
 
-  class ByteReader {
-    ghost var Repr: set<object>
-    var memReader: MemoryReader<uint8>
-
-    predicate Valid()
-      reads this, Repr
+  method ReadBytes(iter: SeqIter<uint8>, n: nat) returns (res: Result<seq<uint8>>)
+    requires n > 0
+    requires iter.Valid()
+    modifies iter, iter._new, iter._modifies
+    ensures res.Success? ==> |res.value| == n
+  {
+    var bytes := [];
+    var i := 0;
+    var more := true;
+    while i < n
+      invariant 0 <= i <= n
+      invariant i == |bytes|
+      invariant iter.Valid() && fresh(iter._new)
     {
-      this in Repr &&
-      (memReader in Repr && memReader.Repr <= Repr && memReader.Valid())
+      more := iter.MoveNext();
+      if (!more) { return Failure("IO Error: Not enough bytes left on stream."); }
+      bytes := bytes + [iter.x];
+      i := i + 1;
     }
+    return Success(bytes);
+  }
 
-    constructor(m: MemoryReader<uint8>)
-      requires m.Valid()
-      ensures memReader == m
-      ensures Valid()
-    {
-      memReader := m;
-      Repr := {this} + {m} + m.Repr;
-    }
+  method ReadByte(iter: SeqIter<uint8>) returns (res: Result<uint8>)
+    requires iter.Valid()
+    modifies iter, iter._new, iter._modifies
+  {
+    var readBytes :- ReadBytes(iter, 1);
+    assert |readBytes| == 1;
+    return Success(readBytes[0]);
+  }
 
-    method ReadByte() returns (res: Result<uint8>)
-      requires Valid()
-      modifies Repr
-      ensures res.Failure? ==> |memReader.data| - memReader.pos < 1
-      ensures Valid()
-      ensures fresh(Repr - old(Repr))
-    {
-      var bytes :- memReader.ReadExact(1);
-      assert |bytes| == 1;
-      Repr := Repr + {memReader} + memReader.Repr;
-      return Success(bytes[0]);
-    }
+  method ReadUInt16(iter: SeqIter<uint8>) returns (res: Result<uint16>)
+    requires iter.Valid()
+    modifies iter, iter._new, iter._modifies
+  {
+    var readBytes :- ReadBytes(iter, 2);
+    assert |readBytes| == 2;
+    var n := SeqToUInt16(readBytes);
+    return Success(n);
+  }
 
-    method ReadBytes(n: nat) returns (res: Result<seq<uint8>>)
-      requires Valid()
-      modifies Repr
-      ensures res.Failure? ==> |memReader.data| - memReader.pos < n
-      ensures res.Success? ==> |res.value| == n
-      ensures Valid()
-      ensures fresh(Repr - old(Repr))
-    {
-      var bytes :- memReader.ReadExact(n);
-      Repr := Repr + {memReader} + memReader.Repr;
-      return Success(bytes);
-    }
-
-    method ReadUInt16() returns (res: Result<uint16>)
-      requires Valid()
-      modifies Repr
-      ensures res.Failure? ==> |memReader.data| - memReader.pos < 2
-      ensures Valid()
-      ensures fresh(Repr - old(Repr))
-    {
-      var bytes :- memReader.ReadExact(2);
-      var n := SeqToUInt16(bytes);
-      Repr := Repr + {memReader} + memReader.Repr;
-      return Success(n);
-    }
-
-    method ReadUInt32() returns (res: Result<uint32>)
-      requires Valid()
-      modifies Repr
-      ensures res.Failure? ==> |memReader.data| - memReader.pos < 4
-      ensures Valid()
-      ensures fresh(Repr - old(Repr))
-    {
-      var bytes :- memReader.ReadExact(4);
-      var n := SeqToUInt32(bytes);
-      Repr := Repr + {memReader} + memReader.Repr;
-      return Success(n);
-    }
-
-    function method GetRemainingCapacity(): (n: nat)
-      reads Repr
-      requires Valid()
-      ensures Valid()
-      ensures n == |memReader.data| - memReader.pos
-    {
-      |memReader.data| - memReader.pos
-    }
-
-    function method GetUsedCapacity(): (n: nat)
-      reads Repr
-      requires Valid()
-      ensures Valid()
-      ensures n == memReader.pos
-    {
-      memReader.pos
-    }
+  method ReadUInt32(iter: SeqIter<uint8>) returns (res: Result<uint32>)
+    requires iter.Valid()
+    modifies iter, iter._new, iter._modifies
+  {
+    var readBytes :- ReadBytes(iter, 4);
+    assert |readBytes| == 4;
+    var n := SeqToUInt32(readBytes);
+    return Success(n);
   }
 
   class StringWriter {
